new/proof/marshal.v
@@ -1,0 +1,672 @@
+From Perennial.Helpers Require Import List.
+
+From New.code.github_com.tchajed Require Import marshal.
+From Perennial.goose_lang.lib Require Import encoding.
+
+From New.proof Require Import proof_prelude.
+
+Notation encoded_length r := (length r) (only parsing).
+Notation encode r := (r) (only parsing).
+
+#[local] Open Scope Z.
+
+Definition has_encoding (data: list u8) (r: list u8) :=
+  r `prefix_of` data.
+
+Typeclasses Opaque has_encoding.
+
+Lemma has_encoding_length {data r} :
+  has_encoding data r →
+  (length r ≤ length data)%nat.
+Proof.
+  rewrite /has_encoding.
+  intros H%prefix_length => //.
+Qed.
+
+Lemma has_encoding_app_characterization data r :
+  has_encoding data r ↔
+  ∃ extra, data = encode r ++ extra.
+Proof.
+  rewrite /has_encoding /prefix //.
+Qed.
+
+Section goose_lang.
+Context `{hG: heapGS Σ, !ffi_semantics _ _, !ext_types _}.
+
+Implicit Types (v:val).
+
+Definition is_enc (enc_v:val) (sz:Z) (r: list val) (remaining: Z) : iProp Σ :=
+  ∃ (s: slice.t) (off_l: loc) (data: list val),
+    let off := Z.of_nat (length r) in
+    "->" ∷ ⌜enc_v = struct.val Enc [("b" ::= slice.val s)%V; ("off" ::= #off_l)%V]⌝ ∗
+    "Hs" ∷ own_slice s byteT (DfracOwn 1) data ∗
+    "Hs_cap" ∷ own_slice_cap s byteT ∗
+    "%Hsz" ∷ ⌜length data = Z.to_nat sz⌝ ∗
+    "%Hremaining" ∷ ⌜(off + remaining)%Z = sz⌝ ∗
+    "enc_off" ∷ off_l ↦[uint64T] #off ∗
+    "%Hoff" ∷ ⌜0 ≤ off ≤ Z.of_nat (length data)⌝ ∗
+    "%Hencoded" ∷ ⌜r `prefix_of` data⌝
+.
+
+Theorem wp_new_enc_from_slice stk E s (data: list val) :
+  {{{ own_slice s byteT (DfracOwn 1) data ∗ own_slice_cap s byteT }}}
+    NewEncFromSlice (slice.val s) @ stk; E
+  {{{ (enc_v:val), RET enc_v; is_enc enc_v (length data) [] (length data) }}}.
+Proof.
+  iIntros (Φ) "[Hs Hcap] HΦ".
+  wp_call.
+  wp_alloc s_l as "s".
+  wp_pures.
+  wp_alloc off_l as "off".
+  wp_load.
+  wp_pures.
+  iModIntro.
+  iApply "HΦ".
+  iExists _, _, _; rewrite /named; iFrame.
+  rewrite nil_length.
+  iSplit; first by eauto.
+  iSplit.
+  { iPureIntro.
+    lia. }
+  iSplit.
+  { iPureIntro. lia. }
+  iSplitL "off".
+  { rewrite zero_val_unseal //=. }
+  iPureIntro.
+  split; first lia.
+  apply prefix_nil.
+Qed.
+
+Theorem wp_new_enc stk E (sz: u64) :
+  {{{ True }}}
+    NewEnc #sz @ stk; E
+  {{{ (enc_v:val), RET enc_v; is_enc enc_v (uint.Z sz) [] (uint.Z sz) }}}.
+Proof.
+  iIntros (Φ) "_ HΦ".
+  wp_call.
+  wp_alloc sz_l as "sz"; wp_pures.
+  wp_alloc b_l as "b"; wp_pures.
+  rewrite zero_val_unseal //=.
+  wp_load.
+  wp_apply wp_slice_make2; iIntros (s) "[Hs Hcap]"; wp_pures.
+  wp_store; wp_pures.
+  wp_load.
+  wp_apply (wp_new_enc_from_slice with "[$Hs $Hcap]").
+  iIntros (v) "Henc"; wp_pures.
+  rewrite replicate_length.
+  iModIntro.
+  iApply "HΦ".
+  iExactEq "Henc".
+  f_equal; word.
+Qed.
+
+(* TODO: I thought there was already a way to do this *)
+Lemma decide_reflect `{!Decision P} :
+  (if decide P then True else False) → P.
+Proof.
+  destruct (decide P); intuition auto.
+Qed.
+Ltac decide_reflect :=
+  apply decide_reflect;
+  first [ vm_compute; exact I | fail "goal is false" ].
+
+Theorem wp_Enc__PutInt stk E enc_v sz r (x:u64) remaining :
+  8 ≤ remaining →
+  {{{ is_enc enc_v sz r remaining }}}
+    Enc__PutInt enc_v #x @ stk; E
+  {{{ RET #(); is_enc enc_v sz (r ++ u64_le_bytes x) (remaining - 8) }}}.
+Proof.
+  iIntros (Hspace Φ) "Hpre HΦ"; iNamed "Hpre".
+  set (off:=length r) in *.
+  wp_call; wp_pures.
+  wp_alloc enc_l as "enc"; wp_pures.
+  wp_alloc x_l as "x".
+  wp_pures.
+  wp_alloc off_l' as "off"; wp_pures.
+  iApply struct_fields_split in "enc"; eauto.
+  { constructor. compute.
+    decide_reflect. }
+  rewrite /struct_fields struct.val_unseal /struct.val_def /= /append.
+  iNamed "enc".
+  repeat (wp_load || wp_pures || wp_store).
+
+  (* TODO: finish porting this proof *)
+
+  (*
+  wp_apply wp_SliceSkip.
+  { word. }
+  iDestruct (own_slice_small_take_drop _ _ _ (W64 off) with "Hs") as "[Hs2 Hs1]".
+  { word. }
+  replace (uint.nat (W64 off)) with off by word.
+  wp_apply (wp_UInt64Put with "Hs2").
+  { len. }
+  iIntros "Hs2".
+  iDestruct (slice.own_slice_combine with "Hs1 Hs2") as "Hs"; first len.
+  wp_pures.
+  wp_load; wp_store.
+  rewrite -fmap_drop drop_drop.
+  iApply "HΦ".
+  iExists _, _, _; iFrame.
+  change (u64_le_bytes x) with (into_val.to_val (V:=u8) <$> u64_le x).
+  rewrite -!fmap_app.
+  iSplitR; first eauto.
+  iFrame "Hs". iModIntro.
+  rewrite encoded_length_app1.
+  change (length (encode1 (EncUInt64 x))) with 8%nat.
+  iSplitR; first by iPureIntro; len.
+  iSplitR; first by iPureIntro; len.
+  iSplitL "Hoff".
+  { iExactEq "Hoff".
+    rewrite /named.
+    repeat (f_equal; try word). }
+  iPureIntro; split.
+  - len.
+  - subst off.
+    apply has_encoding_app; auto.
+    eapply has_encoding_from_app; eauto.
+*)
+Admitted.
+
+(* TODO: finish porting the file *)
+
+(*
+Theorem wp_Enc__PutInt32 stk E enc_v sz r (x:u32) remaining :
+  4 ≤ remaining →
+  {{{ is_enc enc_v sz r remaining }}}
+    Enc__PutInt32 enc_v #x @ stk; E
+  {{{ RET #(); is_enc enc_v sz (r ++ [EncUInt32 x]) (remaining - 4) }}}.
+Proof.
+  iIntros (Hspace Φ) "Hpre HΦ"; iNamed "Hpre".
+  set (off:=encoded_length r) in *.
+  wp_call.
+  wp_load.
+  wp_pures.
+  iDestruct (own_slice_small_sz with "Hs") as %Hslice_len.
+  wp_apply wp_SliceSkip.
+  { word. }
+  iDestruct (own_slice_small_take_drop _ _ _ (W64 off) with "Hs") as "[Hs2 Hs1]".
+  { word. }
+  replace (uint.nat (W64 off)) with off by word.
+  wp_apply (wp_UInt32Put with "Hs2").
+  { len. }
+  iIntros "Hs2".
+  iDestruct (slice.own_slice_combine with "Hs1 Hs2") as "Hs"; first len.
+  wp_pures.
+  wp_load; wp_store.
+  rewrite -fmap_drop drop_drop.
+  iApply "HΦ".
+  iExists _, _, _; iFrame.
+  change (u32_le_bytes x) with (into_val.to_val <$> u32_le x).
+  rewrite -!fmap_app.
+  iSplitR; first eauto.
+  iFrame "Hs". iModIntro.
+  rewrite encoded_length_app1.
+  change (length (encode1 _)) with 4%nat.
+  iSplitR; first by iPureIntro; len.
+  iSplitR; first by iPureIntro; len.
+  iSplitL "Hoff".
+  { iExactEq "Hoff".
+    rewrite /named.
+    repeat (f_equal; try word). }
+  iPureIntro; split.
+  - len.
+  - subst off.
+    apply has_encoding_app; auto.
+    eapply has_encoding_from_app; eauto.
+Qed.
+
+Local Lemma wp_bool2byte stk E (x:bool) :
+  {{{ True }}}
+    bool2byte #x @ stk; E
+  {{{ RET #(W8 (if x then 1 else 0))%Z; True }}}.
+Proof.
+  iIntros (Φ) "_ HΦ". wp_lam.
+  destruct x; wp_pures; by iApply "HΦ".
+Qed.
+
+Theorem wp_Enc__PutBool stk E enc_v sz r (x:bool) remaining :
+  1 ≤ remaining →
+  {{{ is_enc enc_v sz r remaining }}}
+    Enc__PutBool enc_v #x @ stk; E
+  {{{ RET #(); is_enc enc_v sz (r ++ [EncBool x]) (remaining - 1) }}}.
+Proof.
+  iIntros (Hspace Φ) "Hpre HΦ"; iNamed "Hpre".
+  set (off:=encoded_length r) in *.
+  wp_call.
+  wp_load.
+  wp_pures.
+  iDestruct (own_slice_small_sz with "Hs") as %Hslice_len.
+  wp_pures.
+  wp_apply wp_bool2byte.
+  set (u:=W8 (if x then 1 else 0)%Z).
+  wp_pures.
+  wp_apply (wp_SliceSet (V:=byte) with "[$Hs]").
+  { iPureIntro. apply lookup_lt_is_Some_2. word. }
+  iIntros "Hs".
+  wp_pures.
+  wp_load. wp_store.
+  iApply "HΦ". iModIntro.
+  iExists _, _, _. iFrame.
+  iSplit; eauto.
+  rewrite insert_length.
+  iSplit; eauto.
+  rewrite encoded_length_app1. simpl.
+  iSplit.
+  { iPureIntro. word. }
+  iSplit.
+  { iExactEq "Hoff". rewrite /named. do 3 f_equal. word. }
+  iPureIntro.
+  split; first word.
+  replace (<[uint.nat off:=u]> data) with
+      (take off data ++ [u] ++ drop (off + 1) data); last first.
+  { rewrite insert_take_drop. 2:word.
+    repeat f_equal; word. }
+  apply has_encoding_app; eauto.
+  eapply has_encoding_from_app; eauto.
+Qed.
+
+Theorem wp_Enc__PutInts stk E enc_v sz r (x_s: Slice.t) q (xs:list u64) remaining :
+  8*(Z.of_nat $ length xs) ≤ remaining →
+  {{{ is_enc enc_v sz r remaining ∗ own_slice_small x_s uint64T q xs }}}
+    Enc__PutInts enc_v (slice_val x_s) @ stk; E
+  {{{ RET #(); is_enc enc_v sz (r ++ (EncUInt64 <$> xs)) (remaining - 8*(Z.of_nat $ length xs)) ∗
+               own_slice_small x_s uint64T q xs }}}.
+Proof.
+  iIntros (Hbound Φ) "[Henc Hxs] HΦ".
+  wp_rec; wp_pures.
+  wp_apply (wp_forSlicePrefix
+              (λ done todo,
+                "Henc" ∷ is_enc enc_v sz
+                        (r ++ (EncUInt64 <$> done))
+                        (remaining - 8*(Z.of_nat $ length done)))%I
+           with "[] [$Hxs Henc]").
+  - clear Φ.
+    iIntros (???? Hdonetodo) "!>".
+    iIntros (Φ) "HI HΦ"; iNamed "HI".
+    wp_pures.
+    wp_apply (wp_Enc__PutInt with "Henc").
+    { apply (f_equal length) in Hdonetodo; move: Hdonetodo; len. }
+    iIntros "Henc".
+    iApply "HΦ".
+    iExactEq "Henc".
+    rewrite /named; f_equal; len.
+    rewrite fmap_app.
+    rewrite -!app_assoc.
+    reflexivity.
+  - iExactEq "Henc".
+    rewrite /named; f_equal; len.
+    rewrite app_nil_r //.
+  - iIntros "(Hs&HI)"; iNamed "HI".
+    wp_pures. iApply "HΦ"; by iFrame.
+Qed.
+
+Hint Rewrite encoded_length_app1 : len.
+
+Theorem wp_Enc__PutBytes stk E enc_v r sz remaining b_s q bs :
+  Z.of_nat (length bs) ≤ remaining →
+  {{{ is_enc enc_v sz r remaining ∗ own_slice_small b_s byteT q bs }}}
+    Enc__PutBytes enc_v (slice_val b_s) @ stk; E
+  {{{ RET #(); is_enc enc_v sz (r ++ [EncBytes bs]) (remaining - Z.of_nat (length bs)) ∗
+               own_slice_small b_s byteT q bs }}}.
+Proof.
+  iIntros (Hbound Φ) "[Henc Hbs] HΦ"; iNamed "Henc".
+  wp_call.
+  wp_load; wp_pures.
+  iDestruct (own_slice_small_sz with "Hs") as %Hs_sz.
+  wp_apply wp_SliceSkip.
+  { len. }
+  iDestruct (slice_small_split _ (W64 (encoded_length r)) with "Hs") as "[Hs1 Hs2]"; first by len.
+  wp_apply (wp_SliceCopy (V:=byte) with "[$Hbs $Hs2]"); first by len.
+  iIntros "[Hbs Hs2]".
+  iDestruct (own_slice_combine with "Hs1 Hs2") as "Hs"; first by len.
+  wp_pures.
+  wp_load; wp_store.
+  iApply "HΦ".
+  iFrame. iModIntro.
+  iExists _; iSplitR; first by eauto.
+  iSplitR.
+  { iPureIntro; len. }
+  iSplitR.
+  { iPureIntro; len. simpl; len. }
+  iSplitL "Hoff".
+  { iExactEq "Hoff".
+    rewrite /named.
+    f_equal.
+    f_equal.
+    f_equal.
+    len.
+    simpl.
+    word.
+  }
+  iPureIntro.
+  split_and.
+  - len.
+    simpl; len.
+  - replace (uint.nat (W64 (encoded_length r))) with (encoded_length r) by word.
+    rewrite Hencoded.
+    rewrite app_assoc.
+    eapply has_encoding_from_app.
+    rewrite encode_app encode_singleton //=.
+Qed.
+
+Theorem wp_Enc__Finish stk E enc_v r sz remaining :
+  {{{ is_enc enc_v sz r remaining }}}
+    Enc__Finish enc_v @ stk; E
+  {{{ s data, RET slice_val s; ⌜has_encoding data r⌝ ∗
+                               ⌜length data = Z.to_nat sz⌝ ∗
+                               own_slice s byteT (DfracOwn 1) data }}}.
+Proof.
+  iIntros (Φ) "Henc HΦ"; iNamed "Henc"; subst.
+  wp_call.
+  iApply "HΦ"; by iFrame "∗ %".
+Qed.
+
+Definition is_dec (dec_v:val) (r:Rec) (s:Slice.t) (q:dfrac) (data: list u8): iProp Σ :=
+  ∃ (off_l:loc) (off: u64),
+    "->" ∷ ⌜dec_v = (slice_val s, (#off_l, #()))%V⌝ ∗
+    "Hoff" ∷ off_l ↦[uint64T] #off ∗
+    "%Hoff" ∷ ⌜uint.nat off ≤ length data⌝ ∗
+    "Hs" ∷ own_slice_small s byteT q data ∗
+    "%Henc" ∷ ⌜has_encoding (drop (uint.nat off) data) r⌝.
+
+Lemma is_dec_to_own_slice_small dec_v r s q data :
+  is_dec dec_v r s q data -∗
+  own_slice_small s byteT q data.
+Proof.
+  iIntros "H". iNamed "H". iFrame.
+Qed.
+
+Theorem wp_new_dec stk E s q data r :
+  has_encoding data r →
+  {{{ own_slice_small s byteT q data }}}
+    NewDec (slice_val s) @ stk; E
+  {{{ dec_v, RET dec_v; is_dec dec_v r s q data }}}.
+Proof.
+  iIntros (Henc Φ) "Hs HΦ".
+  wp_call.
+  wp_apply (typed_mem.wp_AllocAt uint64T); eauto.
+  iIntros (off_l) "Hoff".
+  wp_pures.
+  iApply "HΦ".
+  iExists _, _; iFrame.
+  iPureIntro.
+  split_and!; auto; len.
+Qed.
+
+Hint Rewrite encoded_length_singleton : len.
+
+Lemma encoded_length_cons x r :
+  encoded_length (x::r) = (length (encode1 x) + encoded_length r)%nat.
+Proof. rewrite encode_cons; len. Qed.
+
+Theorem wp_Dec__GetInt stk E dec_v (x: u64) r s q data :
+  {{{ is_dec dec_v (EncUInt64 x :: r) s q data }}}
+    Dec__GetInt dec_v @ stk; E
+  {{{ RET #x; is_dec dec_v r s q data }}}.
+Proof.
+  iIntros (Φ) "Hdec HΦ"; iNamed "Hdec".
+  wp_call.
+  wp_load; wp_pures.
+  wp_load; wp_store.
+  iDestruct (own_slice_small_sz with "Hs") as %Hsz.
+  wp_apply wp_SliceSkip.
+  { word. }
+  iDestruct (slice.slice_small_split _ off with "Hs") as "[Hs1 Hs2]".
+  { len. }
+  wp_apply (wp_UInt64Get_unchanged with "Hs2").
+  { eapply has_encoding_inv in Henc as [extra [Henc ?]].
+    rewrite -fmap_drop -fmap_take.
+    rewrite Henc.
+    reflexivity. }
+  iIntros "Hs2".
+  iDestruct (slice.own_slice_small_take_drop_1 with "[$Hs1 $Hs2]") as "Hs"; first by word.
+  iApply "HΦ".
+  iExists _, _; iFrame.
+  iSplitR; first by auto.
+  pose proof (has_encoding_length Henc).
+  autorewrite with len in H.
+  rewrite encoded_length_cons in H.
+  change (length (encode1 _)) with 8%nat in H.
+  iSplitR; first iPureIntro.
+  { word. }
+  iPureIntro.
+  replace (uint.nat (word.add off 8)) with (uint.nat off + 8)%nat by word.
+  rewrite -drop_drop.
+  apply has_encoding_inv in Henc as [extra [Henc ?]].
+  rewrite Henc.
+  rewrite encode_cons.
+  eapply has_encoding_from_app.
+  rewrite -app_assoc.
+  rewrite drop_app_ge //.
+Qed.
+
+Theorem wp_Dec__GetInt32 stk E dec_v (x: u32) r s q data :
+  {{{ is_dec dec_v (EncUInt32 x :: r) s q data }}}
+    Dec__GetInt32 dec_v @ stk; E
+  {{{ RET #x; is_dec dec_v r s q data }}}.
+Proof.
+  iIntros (Φ) "Hdec HΦ"; iNamed "Hdec".
+  wp_call.
+  wp_load; wp_pures.
+  wp_load; wp_store.
+  iDestruct (own_slice_small_sz with "Hs") as %Hsz.
+  wp_apply wp_SliceSkip.
+  { word. }
+  iDestruct (slice.slice_small_split _ off with "Hs") as "[Hs1 Hs2]".
+  { len. }
+  wp_apply (wp_UInt32Get_unchanged with "Hs2").
+  { eapply has_encoding_inv in Henc as [extra [Henc ?]].
+    rewrite -fmap_drop -fmap_take.
+    rewrite Henc.
+    reflexivity. }
+  iIntros "Hs2".
+  iDestruct (slice.own_slice_small_take_drop_1 with "[$Hs1 $Hs2]") as "Hs"; first by word.
+  iApply "HΦ".
+  iExists _, _; iFrame.
+  iSplitR; first by auto.
+  pose proof (has_encoding_length Henc).
+  autorewrite with len in H.
+  rewrite encoded_length_cons in H.
+  change (length (encode1 _)) with 4%nat in H.
+  iSplitR; first iPureIntro.
+  { word. }
+  iPureIntro.
+  replace (uint.nat (word.add off 4)) with (uint.nat off + 4)%nat by word.
+  rewrite -drop_drop.
+  apply has_encoding_inv in Henc as [extra [Henc ?]].
+  rewrite Henc.
+  rewrite encode_cons.
+  eapply has_encoding_from_app.
+  rewrite -app_assoc.
+  rewrite drop_app_ge //.
+Qed.
+
+Theorem wp_Dec__GetBool stk E dec_v (x: bool) r s q data :
+  {{{ is_dec dec_v (EncBool x :: r) s q data }}}
+    Dec__GetBool dec_v @ stk; E
+  {{{ RET #x; is_dec dec_v r s q data }}}.
+Proof.
+  iIntros (Φ) "Hdec HΦ"; iNamed "Hdec".
+  wp_call.
+  wp_load; wp_pures.
+  wp_load; wp_store.
+  iDestruct (own_slice_small_sz with "Hs") as %Hsz.
+  pose proof (has_encoding_length Henc).
+  autorewrite with len in H.
+  rewrite encoded_length_cons in H.
+  change (length (encode1 _)) with 1%nat in H.
+  apply has_encoding_inv in Henc as [extra [Henc ?]].
+  rewrite encode_cons in Henc.
+  assert (drop (uint.nat off) data !! 0%nat = Some $ W8 (if x then 1 else 0)) as Hx.
+  { rewrite Henc. done. }
+  rewrite lookup_drop Nat.add_0_r in Hx.
+  wp_apply (wp_SliceGet (V:=byte) with "[$Hs]").
+  { done. }
+  iIntros "Hl". wp_pures.
+  destruct x; wp_pures; iApply "HΦ";
+    iExists _, _; iFrame; iPureIntro.
+  - split; first done.
+    split; first word.
+    eapply has_encoding_from_app.
+    replace (uint.nat (word.add off 1)) with (uint.nat off + 1)%nat by word.
+    rewrite -drop_drop.
+    rewrite Henc /= drop_0 //.
+  - split; first done.
+    split; first word.
+    eapply has_encoding_from_app.
+    replace (uint.nat (word.add off 1)) with (uint.nat off + 1)%nat by word.
+    rewrite -drop_drop.
+    rewrite Henc /= drop_0 //.
+Qed.
+
+(* This version of GetBytes consumes full ownership of the decoder to be able to
+   give the full fraction to the returned slice *)
+Theorem wp_Dec__GetBytes' stk E dec_v bs (n: u64) r s data :
+  n = W64 (length bs) →
+  {{{ is_dec dec_v (EncBytes bs :: r) s (DfracOwn 1) data ∗
+      (∀ vs' : list u8, own_slice_small s byteT (DfracOwn 1) vs' -∗ own_slice s byteT (DfracOwn 1) vs') }}}
+    Dec__GetBytes dec_v #n @ stk; E
+  {{{ s', RET slice_val s'; own_slice s' byteT (DfracOwn 1) bs }}}.
+Proof.
+  iIntros (-> Φ) "(Hdec&Hclo) HΦ"; iNamed "Hdec".
+  pose proof (has_encoding_length Henc).
+  autorewrite with len in H.
+  rewrite encoded_length_cons /= in H.
+  wp_call.
+  wp_load.
+  iDestruct (own_slice_small_sz with "Hs") as %Hsz.
+  wp_pures.
+  iDestruct ("Hclo" with "[$]") as "Hs".
+  wp_apply (wp_SliceSubslice_full with "Hs"); first by word.
+  iIntros (s') "Hbs".
+  wp_pures.
+  wp_load; wp_store.
+  iApply "HΦ". iModIntro.
+  apply has_encoding_inv in Henc as [extra [Hdataeq _]].
+  rewrite encode_cons /= -app_assoc in Hdataeq.
+  iExactEq "Hbs".
+  f_equal.
+  rewrite -> subslice_drop_take by word.
+  replace (uint.nat (word.add off (length bs)) - uint.nat off)%nat with (length bs) by word.
+  rewrite Hdataeq.
+  rewrite take_app_length' //; lia.
+Qed.
+
+Theorem wp_Dec__GetBytes stk E dec_v bs (n: u64) r s q data :
+  n = W64 (length bs) →
+  {{{ is_dec dec_v (EncBytes bs :: r) s q data }}}
+    Dec__GetBytes dec_v #n @ stk; E
+  {{{ q' s', RET slice_val s'; own_slice_small s' byteT q' bs ∗ is_dec dec_v r s q' data }}}.
+Proof.
+  iIntros (-> Φ) "Hdec HΦ"; iNamed "Hdec".
+  pose proof (has_encoding_length Henc).
+  autorewrite with len in H.
+  rewrite encoded_length_cons /= in H.
+  wp_call.
+  wp_load.
+  iDestruct (own_slice_small_sz with "Hs") as %Hsz.
+  iMod (own_slice_small_persist with "Hs") as "#Hs".
+  wp_pures.
+  wp_apply (wp_SliceSubslice_small with "Hs"); first by word.
+  iIntros (s') "Hbs".
+  wp_pures.
+  wp_load; wp_store.
+  iApply "HΦ". iModIntro.
+  apply has_encoding_inv in Henc as [extra [Hdataeq _]].
+  rewrite encode_cons /= -app_assoc in Hdataeq.
+  iSplitL "Hbs".
+  { iExactEq "Hbs".
+    f_equal.
+    rewrite -> subslice_drop_take by word.
+    replace (uint.nat (word.add off (length bs)) - uint.nat off)%nat with (length bs) by word.
+    rewrite Hdataeq.
+    rewrite take_app_length' //; lia.
+  }
+  iExists _, _; iFrame "∗#".
+  iPureIntro.
+  split_and!; auto; try len.
+  replace (uint.nat (word.add off (length bs))) with (uint.nat off + uint.nat (length bs))%nat by word.
+  rewrite -drop_drop.
+  eapply has_encoding_from_app.
+  rewrite Hdataeq.
+  rewrite drop_app_length' //; word.
+Qed.
+
+(* TODO: use this to replace list_lookup_lt (it's much easier to remember) *)
+Local Tactic Notation "list_elem" constr(l) constr(i) "as" simple_intropattern(x) :=
+  let H := fresh "H" x "_lookup" in
+  let i := lazymatch type of i with
+           | nat => i
+           | Z => constr:(Z.to_nat i)
+           | u64 => constr:(uint.nat i)
+           end in
+  destruct (list_lookup_lt _ l i) as [x H];
+  [ try solve [ len ]
+  | ].
+
+Theorem wp_Dec__GetInts stk E dec_v (xs: list u64) r (n: u64) s q data :
+  length xs = uint.nat n →
+  {{{ is_dec dec_v ((EncUInt64 <$> xs) ++ r) s q data }}}
+    Dec__GetInts dec_v #n @ stk; E
+  {{{ (s':Slice.t), RET slice_val s'; is_dec dec_v r s q data ∗ own_slice s' uint64T (DfracOwn 1) xs }}}.
+Proof.
+  iIntros (Hlen Φ) "Hdec HΦ".
+  wp_rec; wp_pures.
+  wp_apply (typed_mem.wp_AllocAt (slice.T uint64T)).
+  { apply zero_val_ty', has_zero_slice_T. }
+  iIntros (s_l) "Hsptr".
+  wp_pures.
+  wp_apply wp_ref_to; auto.
+  iIntros (i_l) "Hi".
+  wp_pures.
+  wp_apply (wp_forUpto (λ i,
+                        let done := take (uint.nat i) xs in
+                        let todo := drop (uint.nat i) xs in
+                        "Hdec" ∷ is_dec dec_v ((EncUInt64 <$> todo) ++ r) s q data ∗
+                        "*" ∷ ∃ s, "Hsptr" ∷ s_l ↦[slice.T uint64T] (slice_val s) ∗
+                                   "Hdone" ∷ own_slice s uint64T (DfracOwn 1) done
+           )%I with "[] [Hi Hsptr Hdec]").
+  - word.
+  - clear Φ.
+    iIntros (?) "!>".
+    iIntros (Φ) "(HI&Hi&%Hlt) HΦ"; iNamed "HI".
+    wp_pures.
+    list_elem xs i as x.
+    rewrite (drop_S _ _ _ Hx_lookup) /=.
+    wp_apply (wp_Dec__GetInt with "Hdec"); iIntros "Hdec".
+    wp_load.
+    wp_apply (wp_SliceAppend with "Hdone"); iIntros (s') "Hdone".
+    wp_store.
+    iApply "HΦ". iFrame "Hsptr".
+    replace (uint.nat (word.add i 1)) with (S (uint.nat i)) by word.
+    erewrite take_S_r; eauto. by iFrame.
+  - rewrite drop_0. iFrame "Hdec Hi".
+    iExists Slice.nil.
+    iFrame.
+    rewrite take_0.
+    iApply own_slice_nil; auto.
+  - iIntros "(HI&Hi)"; iNamed "HI".
+    wp_load.
+    iApply "HΦ".
+    rewrite -> take_ge, drop_ge by len.
+    by iFrame "Hdone Hdec".
+Qed.
+
+(* special case where GetInts is the last thing and there are no more remaining
+items to decode *)
+Theorem wp_Dec__GetInts_complete stk E dec_v (xs: list u64) (n: u64) s q data :
+  length xs = uint.nat n →
+  {{{ is_dec dec_v (EncUInt64 <$> xs) s q data }}}
+    Dec__GetInts dec_v #n @ stk; E
+  {{{ (s':Slice.t), RET slice_val s'; is_dec dec_v [] s q data ∗ own_slice s' uint64T (DfracOwn 1) xs }}}.
+Proof.
+  iIntros (? Φ) "Hpre HΦ".
+  wp_apply (wp_Dec__GetInts _ _ _ _ [] with "[Hpre]"); first by eauto.
+  - rewrite app_nil_r //.
+  - auto.
+Qed.
+*)
+
+End goose_lang.
+
+Typeclasses Opaque has_encoding.
