src/ShouldBuild.v
@@ -100,4 +100,4 @@ From Perennial.program_proof.tutorial Require
 
 From Perennial.program_proof.cachekv Require proof.
 
-From New.proof Require asyncfile append_log.
+From New.proof Require asyncfile append_log marshal.
